Object_Model.thy
@@ -6,7 +6,6 @@
 section \<open>Object Model\label{sec:object-model}\<close>
 theory Object_Model
   imports "HOL-Library.Extended_Nat" Finite_Map_Ext
-    OCL_Types (*"HOL-Library.Transitive_Closure_Table"*)
 begin
 
 text \<open>
@@ -22,7 +21,6 @@ type_synonym assoc = String.literal
 type_synonym role = String.literal
 type_synonym oper = String.literal
 type_synonym param = String.literal
-(*type_synonym enum = String.literal*)
 type_synonym elit = String.literal
 
 datatype param_dir = In | Out | InOut
@@ -55,6 +53,8 @@ definition "oper_in_params op \<equiv>
 definition "oper_out_params op \<equiv>
   filter (\<lambda>p. param_dir p = Out \<or> param_dir p = InOut) (oper_params op)"
 
+text \<open>
+  The following predicates allows one to access class attributes.\<close>
 
 inductive owned_attribute' where
  "fmlookup attributes \<C> = Some attrs\<^sub>\<C> \<Longrightarrow>
@@ -70,6 +70,8 @@ inductive attribute' where
   owned_attribute' attributes \<D> attr \<tau> \<Longrightarrow>
   attribute' attributes \<C> attr \<D> \<tau>"
 
+text \<open>
+  The following predicates allows one to access association ends.\<close>
 
 inductive role_refer_class where
   "role |\<in>| fmdom ends \<Longrightarrow>
@@ -92,7 +94,6 @@ inductive owned_association_end' where
 | "class_roles associations \<C> from role end \<Longrightarrow>
    owned_association_end' associations \<C> (Some from) role end"
 
-
 inductive class_is_association_source' where
   "owned_association_end' associations \<C> from role end \<Longrightarrow>
    class_is_association_source' associations \<C> from role"
@@ -102,10 +103,18 @@ inductive association_end' where
    owned_association_end' associations \<D> from role end \<Longrightarrow>
    association_end' associations \<C> from role \<D> end"
 
-inductive the_association_end' where
-  "The (\<lambda>(\<D>, end). association_end' associations \<C> from role \<D> end) = (\<D>, end) \<Longrightarrow>
-   the_association_end' associations \<C> from role \<D> end"
+inductive association_end_not_unique where
+  "association_end' associations \<C> from role \<D>' end' \<Longrightarrow>
+   \<D> \<noteq> \<D>' \<or> end \<noteq> end' \<Longrightarrow>
+   association_end_not_unique associations \<C> from role \<D> end"
 
+inductive unique_association_end where
+  "association_end' associations \<C> from role \<D> end \<Longrightarrow>
+   \<not> association_end_not_unique associations \<C> from role \<D> end \<Longrightarrow>
+   unique_association_end associations \<C> from role \<D> end"
+
+text \<open>
+  The following predicates allows one to access association classes.\<close>
 
 inductive referred_by_association_class''' where
   "fmlookup association_classes \<A> = Some assoc \<Longrightarrow>
@@ -124,16 +133,27 @@ inductive referred_by_association_class' where
       association_classes associations \<D> from \<A>) = \<D> \<Longrightarrow>
    referred_by_association_class' association_classes associations \<C> from \<A>"
 
+text \<open>
+  The following predicates allows one to access ends of association classes.\<close>
+
 inductive association_class_end' where
   "fmlookup association_classes \<A> = Some assoc \<Longrightarrow>
    fmlookup associations assoc = Some ends \<Longrightarrow>
    fmlookup ends role = Some end \<Longrightarrow>
    association_class_end' association_classes associations \<A> role end"
 
-inductive the_association_class_end' where
-  "The (\<lambda>end. association_class_end' association_classes associations \<A> role end) = end \<Longrightarrow>
-   the_association_class_end' association_classes associations \<A> role end"
+inductive association_class_end_not_unique where
+  "association_class_end' association_classes associations \<A> role end' \<Longrightarrow>
+   end \<noteq> end' \<Longrightarrow>
+   association_class_end_not_unique association_classes associations \<A> role end"
 
+inductive unique_association_class_end where
+  "association_class_end' association_classes associations \<A> role end \<Longrightarrow>
+   \<not> association_class_end_not_unique association_classes associations \<A> role end \<Longrightarrow>
+   unique_association_class_end association_classes associations \<A> role end"
+
+text \<open>
+  The following predicates allows one to access class operations.\<close>
 
 inductive any_operation' where
   "op |\<in>| fset_of_list operations \<Longrightarrow>
@@ -147,19 +167,33 @@ inductive operation' where
    \<not> oper_static op \<Longrightarrow>
    operation' operations \<tau> name \<pi> op"
 
+inductive operation_not_unique where
+  "operation' operations \<tau> name \<pi> oper' \<Longrightarrow>
+   oper \<noteq> oper' \<Longrightarrow>
+   operation_not_unique operations \<tau> name \<pi> oper"
+
+inductive unique_operation where
+  "operation' operations \<tau> name \<pi> oper \<Longrightarrow>
+   \<not> operation_not_unique operations \<tau> name \<pi> oper \<Longrightarrow>
+   unique_operation operations \<tau> name \<pi> oper"
+
 inductive static_operation' where
   "any_operation' operations \<tau> name \<pi> op \<Longrightarrow>
    oper_static op \<Longrightarrow>
    static_operation' operations \<tau> name \<pi> op"
 
-inductive the_operation' where
-  "The (\<lambda>oper. operation' operations \<tau> op \<pi> oper) = oper \<Longrightarrow>
-   the_operation' operations \<tau> op \<pi> oper"
+inductive static_operation_not_unique where
+  "static_operation' operations \<tau> name \<pi> oper' \<Longrightarrow>
+   oper \<noteq> oper' \<Longrightarrow>
+   static_operation_not_unique operations \<tau> name \<pi> oper"
 
-inductive the_static_operation' where
-  "The (\<lambda>oper. static_operation' operations \<tau> op \<pi> oper) = oper \<Longrightarrow>
-   the_static_operation' operations \<tau> op \<pi> oper"
+inductive unique_static_operation where
+  "static_operation' operations \<tau> name \<pi> oper \<Longrightarrow>
+   \<not> static_operation_not_unique operations \<tau> name \<pi> oper \<Longrightarrow>
+   unique_static_operation operations \<tau> name \<pi> oper"
 
+text \<open>
+  The following predicate allows one to check an enumeration literal for existence.\<close>
 
 inductive has_literal' where
   "fmlookup literals e = Some lits \<Longrightarrow>
@@ -172,10 +206,10 @@ subsection \<open>Definition\<close>
 
 locale object_model =
   fixes attributes :: "'a :: semilattice_sup \<rightharpoonup>\<^sub>f attr \<rightharpoonup>\<^sub>f 't :: order"
-  and associations :: "assoc \<rightharpoonup>\<^sub>f role \<rightharpoonup>\<^sub>f 'a assoc_end"
-  and association_classes :: "'a \<rightharpoonup>\<^sub>f assoc"
-  and operations :: "('t, 'e) oper_spec list"
-  and literals :: "'n \<rightharpoonup>\<^sub>f elit fset"
+    and associations :: "assoc \<rightharpoonup>\<^sub>f role \<rightharpoonup>\<^sub>f 'a assoc_end"
+    and association_classes :: "'a \<rightharpoonup>\<^sub>f assoc"
+    and operations :: "('t, 'e) oper_spec list"
+    and literals :: "'n \<rightharpoonup>\<^sub>f elit fset"
   assumes assoc_end_min_less_eq_max:
     "assoc |\<in>| fmdom associations \<Longrightarrow>
      fmlookup associations assoc = Some ends \<Longrightarrow>
@@ -188,26 +222,50 @@ locale object_model =
 begin
 
 abbreviation "attribute \<equiv> attribute' attributes"
-abbreviation "association_end \<equiv> the_association_end' associations"
+abbreviation "association_end \<equiv> unique_association_end associations"
 abbreviation "referred_by_association_class \<equiv>
   referred_by_association_class' association_classes associations"
 abbreviation "association_class_end \<equiv>
-  the_association_class_end' association_classes associations"
-abbreviation "operation \<equiv> the_operation' operations"
-abbreviation "static_operation \<equiv> the_static_operation' operations"
+  unique_association_class_end association_classes associations"
+abbreviation "operation \<equiv> unique_operation operations"
+abbreviation "static_operation \<equiv> unique_static_operation operations"
 abbreviation "has_literal \<equiv> has_literal' literals"
+
+end
+
+(*** Determinism ************************************************************)
+
+subsection \<open>Determinism\<close>
 
 lemma owned_attribute'_det:
   "owned_attribute' attributes \<C> attr \<tau> \<Longrightarrow>
    owned_attribute' attributes \<C> attr \<sigma> \<Longrightarrow> \<tau> = \<sigma>"
   by (elim owned_attribute'.cases; auto)
 
-lemma attribute_det:
-  "attribute' attributes \<C> attr \<D> \<tau> \<Longrightarrow>
-   attribute' attributes \<C> attr \<E> \<sigma> \<Longrightarrow> \<D> = \<E> \<and> \<tau> = \<sigma>"
+lemma (in object_model) attribute_det:
+  "attribute \<C> attr \<D> \<tau> \<Longrightarrow>
+   attribute \<C> attr \<E> \<sigma> \<Longrightarrow> \<D> = \<E> \<and> \<tau> = \<sigma>"
   by (elim attribute'.cases; auto simp add: owned_attribute'_det)
 
-end
+lemma (in object_model) association_end_det:
+  "association_end \<C> from role \<D>\<^sub>1 end\<^sub>1 \<Longrightarrow>
+   association_end \<C> from role \<D>\<^sub>2 end\<^sub>2 \<Longrightarrow> \<D>\<^sub>1 = \<D>\<^sub>2 \<and> end\<^sub>1 = end\<^sub>2"
+  by (meson association_end_not_unique.intros unique_association_end.cases)
+
+lemma (in object_model) association_class_end_det:
+  "association_class_end \<A> role end\<^sub>1 \<Longrightarrow>
+   association_class_end \<A> role end\<^sub>2 \<Longrightarrow> end\<^sub>1 = end\<^sub>2"
+  by (meson association_class_end_not_unique.intros unique_association_class_end.cases)
+
+lemma (in object_model) operation_det:
+  "operation \<tau> name \<pi> oper\<^sub>1 \<Longrightarrow>
+   operation \<tau> name \<pi> oper\<^sub>2 \<Longrightarrow> oper\<^sub>1 = oper\<^sub>2"
+  by (meson operation_not_unique.intros unique_operation.cases)
+
+lemma (in object_model) static_operation_det:
+  "static_operation \<tau> name \<pi> oper\<^sub>1 \<Longrightarrow>
+   static_operation \<tau> name \<pi> oper\<^sub>2 \<Longrightarrow> oper\<^sub>1 = oper\<^sub>2"
+  by (meson static_operation_not_unique.intros unique_static_operation.cases)
 
 (*** Code Setup *************************************************************)
 
@@ -276,33 +334,22 @@ code_pred (modes:
     i \<Rightarrow> i \<Rightarrow> o \<Rightarrow> o \<Rightarrow> o \<Rightarrow> i \<Rightarrow> bool,
     i \<Rightarrow> i \<Rightarrow> o \<Rightarrow> o \<Rightarrow> o \<Rightarrow> o \<Rightarrow> bool) [show_modes] association_end' .
 
-lemma the_association_end'_code_predI [code_pred_intro]:
-  "Predicate.the (association_end'_i_i_i_i_o_o associations \<C> from role) = (\<D>, end) \<Longrightarrow>
-   the_association_end' associations \<C> from role \<D> end"
-  by (simp add: Predicate.the_def the_association_end'.simps
-       association_end'_i_i_i_i_o_o_def)
+code_pred (modes:
+    i \<Rightarrow> i \<Rightarrow> i \<Rightarrow> i \<Rightarrow> i \<Rightarrow> i \<Rightarrow> bool) [show_modes] association_end_not_unique .
 
 code_pred (modes:
     i \<Rightarrow> i \<Rightarrow> i \<Rightarrow> i \<Rightarrow> i \<Rightarrow> i \<Rightarrow> bool,
     i \<Rightarrow> i \<Rightarrow> i \<Rightarrow> i \<Rightarrow> i \<Rightarrow> o \<Rightarrow> bool,
     i \<Rightarrow> i \<Rightarrow> i \<Rightarrow> i \<Rightarrow> o \<Rightarrow> i \<Rightarrow> bool,
-    i \<Rightarrow> i \<Rightarrow> i \<Rightarrow> i \<Rightarrow> o \<Rightarrow> o \<Rightarrow> bool) [show_modes] the_association_end'
-  by (metis Predicate.the_def association_end'_i_i_i_i_o_o_def pred.sel the_association_end'.cases)
+    i \<Rightarrow> i \<Rightarrow> i \<Rightarrow> i \<Rightarrow> o \<Rightarrow> o \<Rightarrow> bool) [show_modes] unique_association_end .
 
 code_pred [show_modes] referred_by_association_class' .
 
 code_pred [show_modes] association_class_end' .
 
-lemma the_association_class_end'_code_predI [code_pred_intro]:
-  "Predicate.the (association_class_end'_i_i_i_i_o association_classes associations \<A> role) = end \<Longrightarrow>
-   the_association_class_end' association_classes associations \<A> role end"
-  by (simp add: Predicate.the_def the_association_class_end'.simps
-       association_class_end'_i_i_i_i_o_def)
+code_pred [show_modes] association_class_end_not_unique .
 
-code_pred (modes:
-    i \<Rightarrow> i \<Rightarrow> i \<Rightarrow> i \<Rightarrow> i \<Rightarrow> bool,
-    i \<Rightarrow> i \<Rightarrow> i \<Rightarrow> i \<Rightarrow> o \<Rightarrow> bool) [show_modes] the_association_class_end'
-  by (metis the_association_class_end'.cases the_association_class_end'_code_predI)
+code_pred  [show_modes] unique_association_class_end .
 
 code_pred (modes:
     i \<Rightarrow> i \<Rightarrow> i \<Rightarrow> i \<Rightarrow> i \<Rightarrow> bool,
@@ -312,180 +359,24 @@ code_pred (modes:
     i \<Rightarrow> i \<Rightarrow> i \<Rightarrow> i \<Rightarrow> i \<Rightarrow> bool,
     i \<Rightarrow> i \<Rightarrow> i \<Rightarrow> i \<Rightarrow> o \<Rightarrow> bool) [show_modes] operation' .
 
-lemma the_operation'_code_predI [code_pred_intro]:
-  "Predicate.the (operation'_i_i_i_i_o operations \<tau> op \<pi>) = oper \<Longrightarrow>
-   the_operation' operations \<tau> op \<pi> oper"
-  by (simp add: Predicate.the_def the_operation'.simps
-       operation'_i_i_i_i_o_def)
+code_pred (modes:
+    i \<Rightarrow> i \<Rightarrow> i \<Rightarrow> i \<Rightarrow> i \<Rightarrow> bool) [show_modes] operation_not_unique .
 
 code_pred (modes:
     i \<Rightarrow> i \<Rightarrow> i \<Rightarrow> i \<Rightarrow> i \<Rightarrow> bool,
-    i \<Rightarrow> i \<Rightarrow> i \<Rightarrow> i \<Rightarrow> o \<Rightarrow> bool) [show_modes] the_operation'
-  by (metis the_operation'.cases the_operation'_code_predI)
+    i \<Rightarrow> i \<Rightarrow> i \<Rightarrow> i \<Rightarrow> o \<Rightarrow> bool) [show_modes] unique_operation .
 
 code_pred (modes:
     i \<Rightarrow> i \<Rightarrow> i \<Rightarrow> i \<Rightarrow> i \<Rightarrow> bool,
     i \<Rightarrow> i \<Rightarrow> i \<Rightarrow> i \<Rightarrow> o \<Rightarrow> bool) [show_modes] static_operation' .
 
-lemma the_static_operation'_code_predI [code_pred_intro]:
-  "Predicate.the (static_operation'_i_i_i_i_o operations \<tau> op \<pi>) = oper \<Longrightarrow>
-   the_static_operation' operations \<tau> op \<pi> oper"
-  by (simp add: Predicate.the_def the_static_operation'.simps
-       static_operation'_i_i_i_i_o_def)
+code_pred (modes:
+    i \<Rightarrow> i \<Rightarrow> i \<Rightarrow> i \<Rightarrow> i \<Rightarrow> bool) [show_modes] static_operation_not_unique .
 
 code_pred (modes:
     i \<Rightarrow> i \<Rightarrow> i \<Rightarrow> i \<Rightarrow> i \<Rightarrow> bool,
-    i \<Rightarrow> i \<Rightarrow> i \<Rightarrow> i \<Rightarrow> o \<Rightarrow> bool) [show_modes] the_static_operation'
-  by (metis the_static_operation'.cases the_static_operation'_code_predI)
+    i \<Rightarrow> i \<Rightarrow> i \<Rightarrow> i \<Rightarrow> o \<Rightarrow> bool) [show_modes] unique_static_operation .
 
 code_pred [show_modes] has_literal' .
-
-(*
-(*** Classes ****************************************************************)
-
-section \<open>Classes\<close>
-
-datatype classes1 =
-  Object | Person | Employee | Customer | Project | Task | Sprint
-
-inductive subclass1 where
-  "c \<noteq> Object \<Longrightarrow>
-   subclass1 c Object"
-| "subclass1 Employee Person"
-| "subclass1 Customer Person"
-
-code_pred subclass1 .
-
-instantiation classes1 :: semilattice_sup
-begin
-
-definition "(<) \<equiv> subclass1"
-definition "(\<le>) \<equiv> subclass1\<^sup>=\<^sup>="
-
-notation sup (infixl "\<squnion>" 65)
-
-fun sup_classes1 where
-  "Object \<squnion> _ = Object"
-| "Person \<squnion> c = (if c = Person \<or> c = Employee \<or> c = Customer
-    then Person else Object)"
-| "Employee \<squnion> c = (if c = Employee then Employee else
-    if c = Person \<or> c = Customer then Person else Object)"
-| "Customer \<squnion> c = (if c = Customer then Customer else
-    if c = Person \<or> c = Employee then Person else Object)"
-| "Project \<squnion> c = (if c = Project then Project else Object)"
-| "Task \<squnion> c = (if c = Task then Task else Object)"
-| "Sprint \<squnion> c = (if c = Sprint then Sprint else Object)"
-
-lemma less_le_not_le_classes1:
-  "c < d \<longleftrightarrow> c \<le> d \<and> \<not> d \<le> c"
-  for c d :: classes1
-  unfolding less_classes1_def less_eq_classes1_def
-  using subclass1.simps by auto
-
-lemma order_refl_classes1:
-  "c \<le> c"
-  for c :: classes1
-  unfolding less_eq_classes1_def by simp
-
-lemma order_trans_classes1:
-  "c \<le> d \<Longrightarrow> d \<le> e \<Longrightarrow> c \<le> e"
-  for c d e :: classes1
-  unfolding less_eq_classes1_def
-  using subclass1.simps by auto
-
-lemma antisym_classes1:
-  "c \<le> d \<Longrightarrow> d \<le> c \<Longrightarrow> c = d"
-  for c d :: classes1
-  unfolding less_eq_classes1_def
-  using subclass1.simps by auto
-
-lemma sup_ge1_classes1:
-  "c \<le> c \<squnion> d"
-  for c d :: classes1
-  by (induct c; auto simp add: less_eq_classes1_def less_classes1_def subclass1.simps)
-
-lemma sup_ge2_classes1:
-  "d \<le> c \<squnion> d"
-  for c d :: classes1
-  by (induct c; auto simp add: less_eq_classes1_def less_classes1_def subclass1.simps)
-
-lemma sup_least_classes1:
-  "c \<le> e \<Longrightarrow> d \<le> e \<Longrightarrow> c \<squnion> d \<le> e"
-  for c d e :: classes1
-  by (induct c; induct d;
-      auto simp add: less_eq_classes1_def less_classes1_def subclass1.simps)
-
-instance
-  apply intro_classes
-  apply (simp add: less_le_not_le_classes1)
-  apply (simp add: order_refl_classes1)
-  apply (rule order_trans_classes1; auto)
-  apply (simp add: antisym_classes1)
-  apply (simp add: sup_ge1_classes1)
-  apply (simp add: sup_ge2_classes1)
-  apply (simp add: sup_least_classes1)
-  done
-
-end
-
-instantiation classes1 :: enum
-begin
-
-definition [simp]: "enum_classes1 \<equiv>
-  [Object, Person, Employee, Customer, Project, Task, Sprint]"
-
-definition [simp]: "enum_all_classes1 P \<equiv>
-  P Object \<and> P Person \<and> P Employee \<and> P Customer \<and> P Project \<and> P Task \<and> P Sprint"
-
-definition [simp]: "enum_ex_classes1 P \<equiv>
-  P Object \<or> P Person \<or> P Employee \<or> P Customer \<or> P Project \<or> P Task \<or> P Sprint" 
-
-instance
-  apply intro_classes
-  apply auto
-  by (metis classes1.exhaust)+
-
-end
-
-abbreviation "assocs \<equiv> [
-  STR ''ProjectManager'' \<mapsto>\<^sub>f [
-    STR ''projects'' \<mapsto>\<^sub>f (Project, 0::nat, \<infinity>::enat, False, True),
-    STR ''manager'' \<mapsto>\<^sub>f (Employee, 1, 1, False, False)],
-  STR ''ProjectMember'' \<mapsto>\<^sub>f [
-    STR ''member_of'' \<mapsto>\<^sub>f (Project, 0, \<infinity>, False, False),
-    STR ''members'' \<mapsto>\<^sub>f (Employee, 1, 20, True, True)],
-  STR ''ManagerEmployee'' \<mapsto>\<^sub>f [
-    STR ''line_manager'' \<mapsto>\<^sub>f (Employee, 0::nat, 1, False, False),
-    STR ''project_manager'' \<mapsto>\<^sub>f (Employee, 0::nat, \<infinity>, False, False),
-    STR ''employees'' \<mapsto>\<^sub>f (Employee, 3, 7, False, False)],
-  STR ''ProjectCustomer'' \<mapsto>\<^sub>f [
-    STR ''projects'' \<mapsto>\<^sub>f (Project, 0, \<infinity>, False, True),
-    STR ''customer'' \<mapsto>\<^sub>f (Customer, 1, 1, False, False)],
-  STR ''ProjectTask'' \<mapsto>\<^sub>f [
-    STR ''project'' \<mapsto>\<^sub>f (Project, 1, 1, False, False),
-    STR ''tasks'' \<mapsto>\<^sub>f (Task, 0, \<infinity>, True, True)],
-  STR ''SprintTaskAssignee'' \<mapsto>\<^sub>f [
-    STR ''sprint'' \<mapsto>\<^sub>f (Sprint, 0, 10, False, True),
-    STR ''tasks'' \<mapsto>\<^sub>f (Task, 0, 5, False, True),
-    STR ''assignee'' \<mapsto>\<^sub>f (Employee, 0, 1, False, False)]]"
-(*
-definition "operations_classes1 \<equiv> [
-  (STR ''membersCount'', Person, [], 1::nat, False, None :: nat option),
-  (STR ''membersByName'', Project, [(STR ''mn'', 1::nat, In)], 1, False, None),
-  (STR ''allProjects'', Project, [], 1, True, None)
-  ]"
-*)
-declare [[coercion "ObjectType :: classes1 \<Rightarrow> classes1 basic_type"]]
-
-definition "operations_classes1 \<equiv> [
-  (STR ''membersCount'', Project[1], [], Integer[1], False, None),
-  (STR ''membersByName'', Project[1], [(STR ''mn'', String[1], In)], Set Employee[1], False, None),
-  (STR ''allProjects'', Project[1], [], Set Project[1], True, None)
-  ] :: (classes1 type, nat) oper_spec list"
-
-
-value "any_operation' operations_classes1 Employee[1] STR ''membersCount'' [] (STR ''membersCount'', Project[1], [], Integer[1], False, None)"
-values "{op. any_operation' operations_classes1 Employee[1] STR ''membersCount'' [] op}"
-*)
 
 end
