OCL_Normalization.thy
@@ -241,29 +241,30 @@ inductive_cases IteratorCallNE [elim]: "(\<Gamma>, \<tau>) \<turnstile>\<^sub>C 
 inductive_cases ExprListNE [elim]: "\<Gamma> \<turnstile>\<^sub>L xs \<Rrightarrow> ys"
 
 (*** Simplification Rules ***************************************************)
-(*
+
 section \<open>Simplification Rules\<close>
 
-inductive_simps LiteralNS [simp]: "\<Gamma> \<turnstile> Literal a \<Rrightarrow> b"
-inductive_simps LetNS [simp]: "\<Gamma> \<turnstile> Let v t init body \<Rrightarrow> b"
-inductive_simps VarNS [simp]: "\<Gamma> \<turnstile> Var v \<Rrightarrow> b"
-inductive_simps IfNS [simp]: "\<Gamma> \<turnstile> If a b c \<Rrightarrow> d"
+inductive_simps normalize_alt_simps:
+"\<Gamma> \<turnstile> Literal a \<Rrightarrow> b"
+"\<Gamma> \<turnstile> Let v t init body \<Rrightarrow> b"
+"\<Gamma> \<turnstile> Var v \<Rrightarrow> b"
+"\<Gamma> \<turnstile> If a b c \<Rrightarrow> d"
 
-inductive_simps MetaOperationCallNS [simp]: "\<Gamma> \<turnstile> MetaOperationCall \<tau> op \<Rrightarrow> b"
-inductive_simps StaticOperationCallNS [simp]: "\<Gamma> \<turnstile> StaticOperationCall \<tau> op as \<Rrightarrow> b"
-inductive_simps DotCallNS [simp]: "\<Gamma> \<turnstile> Call src DotCall call \<Rrightarrow> b"
-inductive_simps SafeDotCallNS [simp]: "\<Gamma> \<turnstile> Call src SafeDotCall call \<Rrightarrow> b"
-inductive_simps ArrowCallNS [simp]: "\<Gamma> \<turnstile> Call src ArrowCall call \<Rrightarrow> b"
-inductive_simps SafeArrowCallNS [simp]: "\<Gamma> \<turnstile> Call src SafeArrowCall call \<Rrightarrow> b"
+"\<Gamma> \<turnstile> MetaOperationCall \<tau> op \<Rrightarrow> b"
+"\<Gamma> \<turnstile> StaticOperationCall \<tau> op as \<Rrightarrow> b"
+"\<Gamma> \<turnstile> Call src DotCall call \<Rrightarrow> b"
+"\<Gamma> \<turnstile> Call src SafeDotCall call \<Rrightarrow> b"
+"\<Gamma> \<turnstile> Call src ArrowCall call \<Rrightarrow> b"
+"\<Gamma> \<turnstile> Call src SafeArrowCall call \<Rrightarrow> b"
 
-inductive_simps CallNS [simp]: "(\<Gamma>, \<tau>) \<turnstile>\<^sub>C call \<Rrightarrow> b"
-inductive_simps OperationCallNS [simp]: "(\<Gamma>, \<tau>) \<turnstile>\<^sub>C Operation op as \<Rrightarrow> call"
-inductive_simps IterateCallNS [simp]: "(\<Gamma>, \<tau>) \<turnstile>\<^sub>C Iterate its its_ty res res_t res_init body \<Rrightarrow> call"
-inductive_simps IteratorCallNS [simp]: "(\<Gamma>, \<tau>) \<turnstile>\<^sub>C Iterator iter its its_ty body \<Rrightarrow> call"
+"(\<Gamma>, \<tau>) \<turnstile>\<^sub>C call \<Rrightarrow> b"
+"(\<Gamma>, \<tau>) \<turnstile>\<^sub>C Operation op as \<Rrightarrow> call"
+"(\<Gamma>, \<tau>) \<turnstile>\<^sub>C Iterate its its_ty res res_t res_init body \<Rrightarrow> call"
+"(\<Gamma>, \<tau>) \<turnstile>\<^sub>C Iterator iter its its_ty body \<Rrightarrow> call"
 
-inductive_simps ExprListNilNS [simp]: "\<Gamma> \<turnstile>\<^sub>L [] \<Rrightarrow> ys"
-inductive_simps ExprListConsNS [simp]: "\<Gamma> \<turnstile>\<^sub>L x # xs \<Rrightarrow> ys"
-*)
+"\<Gamma> \<turnstile>\<^sub>L [] \<Rrightarrow> ys"
+"\<Gamma> \<turnstile>\<^sub>L x # xs \<Rrightarrow> ys"
+
 (*** Determinism ************************************************************)
 
 section \<open>Determinism\<close>
